ACL2Lean.lean
@@ -1,5 +1,6 @@
 -- Root `ACL2Lean` library entry point.
 import ACL2Lean.Basic
+import ACL2Lean.DSL.SyntaxCategories
 import ACL2Lean.Syntax
 import ACL2Lean.Parser
 import ACL2Lean.Import
@@ -9,5 +10,4 @@ import ACL2Lean.Translator
 import ACL2Lean.Logic
 import ACL2Lean.Tactics
 import ACL2Lean.DSL
-import ACL2Lean.PrettyPrinter
 import ACL2Lean.PrettyPrinter
