ACL2Lean/DSL/SyntaxCategories.lean
@@ -18,6 +18,10 @@ syntax "!" : acl2_id
 syntax "?" : acl2_id
 syntax "if" : acl2_id
 syntax "quote" : acl2_id
+syntax "let" : acl2_id
+syntax "declare" : acl2_id
+-- Support for IDs with hyphens
+syntax ident "-" acl2_id : acl2_id
 
 declare_syntax_cat acl2_sexpr
 syntax acl2_id : acl2_sexpr
@@ -27,10 +31,12 @@ syntax "(" acl2_sexpr* ")" : acl2_sexpr
 syntax ":" acl2_id : acl2_sexpr
 
 declare_syntax_cat acl2_event
-syntax "(" "defun" acl2_id+ "(" acl2_id* ")" acl2_sexpr ")" : acl2_event
-syntax "(" "defthm" acl2_id+ acl2_sexpr (":" term)? ")" : acl2_event
-syntax "(" "defmacro" acl2_id+ "(" acl2_id* ")" acl2_sexpr ")" : acl2_event
+syntax "(" "defun" acl2_id "(" acl2_id* ")" acl2_sexpr* ")" ("termination_by" term)? ("decreasing_by" tacticSeq)? : acl2_event
+syntax "(" "defthm" acl2_id acl2_sexpr ")" (":" term)? : acl2_event
+syntax "(" "defmacro" acl2_id "(" acl2_id* ")" acl2_sexpr ")" : acl2_event
 syntax "(" "defconst" acl2_id acl2_sexpr ")" : acl2_event
+syntax "(" "defrec" acl2_id "(" acl2_id* ")" acl2_sexpr ")" : acl2_event
+syntax "(" "defstobj" acl2_id acl2_sexpr* ")" : acl2_event
 syntax "(" "in-package" str ")" : acl2_event
 syntax "(" "include-book" str ")" : acl2_event
 
