ACL2Lean/PrettyPrinter.lean
@@ -7,51 +7,51 @@ open Lean PrettyPrinter
 namespace ACL2
 
 @[app_unexpander SExpr.nil]
-def unexpandSExprNil : Lean.PrettyPrinter.Unexpander := fun _ =>
+def unexpandSExprNil : Unexpander := fun _ =>
   `(nil)
 
 @[app_unexpander SExpr.atom]
-def unexpandSExprAtom : Lean.PrettyPrinter.Unexpander := fun stx =>
+def unexpandSExprAtom : Unexpander := fun stx =>
   match stx with
   | `($_ $a) => pure a
   | _ => throw ()
 
 @[app_unexpander Atom.bool]
-def unexpandAtomBool : Lean.PrettyPrinter.Unexpander := fun stx =>
+def unexpandAtomBool : Unexpander := fun stx =>
   match stx with
   | `($_ true) => `(t)
   | `($_ false) => `(nil)
   | _ => throw ()
 
 @[app_unexpander Atom.number]
-def unexpandAtomNumber : Lean.PrettyPrinter.Unexpander := fun stx =>
+def unexpandAtomNumber : Unexpander := fun stx =>
   match stx with
   | `($_ $n) => pure n
   | _ => throw ()
 
 @[app_unexpander Number.int]
-def unexpandNumberInt : Lean.PrettyPrinter.Unexpander := fun stx =>
+def unexpandNumberInt : Unexpander := fun stx =>
   match stx with
   | `($_ $n) => pure n
   | _ => throw ()
 
 @[app_unexpander Atom.symbol]
-def unexpandAtomSymbol : Lean.PrettyPrinter.Unexpander := fun stx =>
+def unexpandAtomSymbol : Unexpander := fun stx =>
   match stx with
   | `($_ { package := $_, name := $name }) =>
     match name.raw.isStrLit? with
-    | some s => pure (Lean.mkIdent (Name.mkSimple s))
+    | some s => pure (mkIdent (Name.mkSimple s))
     | none => throw ()
   | _ => throw ()
 
 @[app_unexpander Atom.string]
-def unexpandAtomString : Lean.PrettyPrinter.Unexpander := fun stx =>
+def unexpandAtomString : Unexpander := fun stx =>
   match stx with
   | `($_ $s) => pure s
   | _ => throw ()
 
 @[app_unexpander SExpr.cons]
-def unexpandSExprCons : Lean.PrettyPrinter.Unexpander := fun stx =>
+def unexpandSExprCons : Unexpander := fun stx =>
   match stx with
   | `($_ $car $cdr) =>
     match cdr with
@@ -60,19 +60,19 @@ def unexpandSExprCons : Lean.PrettyPrinter.Unexpander := fun stx =>
   | _ => throw ()
 
 @[app_unexpander Logic.plus]
-def unexpandPlus : Lean.PrettyPrinter.Unexpander := fun stx =>
+def unexpandPlus : Unexpander := fun stx =>
   match stx with
   | `($_ $a $b) => `(plus $a $b)
   | _ => throw ()
 
 @[app_unexpander Logic.equal]
-def unexpandEqual : Lean.PrettyPrinter.Unexpander := fun stx =>
+def unexpandEqual : Unexpander := fun stx =>
   match stx with
   | `($_ $a $b) => `(equal $a $b)
   | _ => throw ()
 
 @[app_unexpander Logic.toBool]
-def unexpandToBool : Lean.PrettyPrinter.Unexpander := fun stx =>
+def unexpandToBool : Unexpander := fun stx =>
   match stx with
   | `($_ $a) => pure a
   | _ => throw ()
